Verfied CSE

dafny/SortBloodVolume.dfy
@@ -24,6 +24,7 @@ class Blood {
   requires v > 0 && u > 0;
   requires l != "" && dn != "" && de != ""
   ensures Valid();
+  modifies this;
   {
     blood_id := id;
     blood_type := b;
@@ -35,58 +36,53 @@ class Blood {
     donor_email := de;
     ordered := o;
   }
-
-  method OrderBlood()
-  requires Valid();
-  ensures Valid();
-  requires ordered == false;
-  ensures ordered == true;
-  modifies this;
-  {
-    ordered := true;
-  }
 }
 
 
-predicate SortedExpiration(a: array?<Blood>, asc: bool)
+predicate SortedVolume(a: array<Blood>, asc: bool)
 requires a != null;
+requires forall j :: 0 <= j < a.Length ==> a[j] != null && a[j].Valid();
 reads a;
 reads set x | x in a[..];
 {
   asc ==> (forall j, k :: 0 <= j <= k < a.Length 
-    ==> a[j].use_by_date <= a[k].use_by_date) &&
+    ==> a[j].volume <= a[k].volume) &&
   !asc ==> (forall j, k :: 0 <= j <= k < a.Length 
-    ==> a[k].use_by_date <= a[j].use_by_date)
+    ==> a[k].volume <= a[j].volume)
 }
 
 
-predicate SortedBetweenExpiration(a: array?<Blood>, asc: bool, lower: int, upper: int)
+predicate SortedBetweenVolume(a: array<Blood>, asc: bool, lower: int, upper: int)
 requires a != null;
+requires forall j :: 0 <= j < a.Length ==> a[j] != null && a[j].Valid();
 requires lower <= upper < a.Length;
 reads a;
 reads set x | x in a[..];
 {
   asc ==> (forall j, k :: 0 <= lower <= j <= k <= upper < a.Length 
-    ==> a[j].use_by_date <= a[k].use_by_date) &&
+    ==> a[j].volume <= a[k].volume) &&
   !asc ==> (forall j, k :: 0 <= lower <= j <= k <= upper < a.Length 
-    ==> a[k].use_by_date <= a[j].use_by_date)
+    ==> a[k].volume <= a[j].volume)
 }
 
 
-predicate PartitionExpiration(a: array?<Blood>, asc: bool, i: int)
+predicate PartitionVolume(a: array<Blood>, asc: bool, i: int)
 requires a != null;
+requires forall j :: 0 <= j < a.Length ==> a[j] != null && a[j].Valid();
 reads a;
 reads set x | x in a[..];
 {
   asc ==> (forall j, k :: 0 <= j <= i < k < a.Length 
-    ==> a[j].use_by_date <= a[k].use_by_date) &&
+    ==> a[j].volume <= a[k].volume) &&
   !asc ==> (forall j, k :: 0 <= j <= i < k < a.Length 
-    ==> a[k].use_by_date <= a[j].use_by_date)
+    ==> a[k].volume <= a[j].volume)
 }
 
 
-method BubbleSortExpiration(a: array?<Blood>, asc: bool)
+method BubbleSortVolume(a: array<Blood>, asc: bool)
 requires a != null;
+requires forall j :: 0 <= j < a.Length ==> a[j] != null && a[j].Valid();
+ensures forall j :: 0 <= j < a.Length ==> a[j] != null && a[j].Valid();
 ensures SortedExpiration(a, asc);
 modifies a;
 {
@@ -95,6 +91,7 @@ modifies a;
   while i > 0
   invariant i < 0 ==> a.Length == 0;
   invariant -1 <= i < a.Length;
+  invariant forall j :: 0 <= j < a.Length ==> a[j] != null && a[j].Valid();
   invariant SortedBetweenExpiration(a, asc, i, a.Length - 1);
   invariant PartitionExpiration(a, asc, i);
   decreases i;
@@ -104,18 +101,19 @@ modifies a;
     while j < i
     decreases i - j;
     invariant 0 < i < a.Length && 0 <= j <= i;
+    invariant forall j :: 0 <= j < a.Length ==> a[j] != null && a[j].Valid();
     invariant asc ==> (forall k :: 0 <= k <= j 
-      ==> a[k].use_by_date <= a[j].use_by_date);
+      ==> a[k].volume <= a[j].volume);
     invariant !asc ==> (forall k :: 0 <= k <= j 
-      ==> a[j].use_by_date <= a[k].use_by_date);
+      ==> a[j].volume <= a[k].volume);
     invariant SortedBetweenExpiration(a, asc, i, a.Length - 1);
     invariant PartitionExpiration(a, asc, i);
-    {
-      if asc && (a[j].use_by_date > a[j + 1].use_by_date)
+    {  
+      if asc && (a[j].volume > a[j + 1].volume)
       {
         a[j], a[j + 1] := a[j + 1], a[j];
       } 
-      else if !asc && (a[j].use_by_date < a[j + 1].use_by_date)
+      else if !asc && (a[j].volume < a[j + 1].volume)
       {
         a[j], a[j + 1] := a[j + 1], a[j];
       }
@@ -127,31 +125,32 @@ modifies a;
   }
 }
 
+
 method Main() 
 {
   var b1 := new Blood(1, AP, 3, true, 100, "UNSW", "John Doe", "Donor01@gmail.com", false);
   var b2 := new Blood(2, AN, 4, true, 90, "UNSW", "Steve Doe", "Donor02@gmail.com", false);
   var b3 := new Blood(3, BN, 8, true, 70, "UNSW", "Kate Doe", "Donor03@gmail.com", false);
 
-  var a := new Blood[][b1, b2, b3];
+  assert b1 != null && b1.Valid();
+  assert b2 != null && b2.Valid();
+  assert b3 != null && b3.Valid();
+
+  var a := new Blood[3];
+  a[0], a[1], a[2] := b2, b1, b3;
+
+  assert a[0] == b2 && a[0] != null && a[0].Valid();
+  assert a[1] == b1 && a[1] != null && a[1].Valid();
+  assert a[2] == b3 && a[2] != null && a[2].Valid();
+  assert forall j :: 0 <= j < a.Length ==> a[j] != null && a[j].Valid();
+  
   BubbleSortExpiration(a, true);
-
   assert SortedExpiration(a, true);
-  print(a[0].blood_id);
-  print(" ");
-  print(a[1].blood_id);
-  print(" ");
-  print(a[2].blood_id);
-  print("\n");
 
-  var b := new Blood[][b2, b1, b3];
-  BubbleSortExpiration(b, false);
+  print a[0].blood_id, " ", a[1].blood_id, " ", a[2].blood_id, "\n";
 
-  assert SortedExpiration(b, false);
-  print(b[0].blood_id);
-  print(" ");
-  print(b[1].blood_id);
-  print(" ");
-  print(b[2].blood_id);
-  print("\n");
+  BubbleSortExpiration(a, false);
+  assert SortedExpiration(a, false);
+
+  print a[0].blood_id, " ", a[1].blood_id, " ", a[2].blood_id, "\n";
 }
